src/MicroSail/SmallStep/Step.v
@@ -45,8 +45,8 @@ Module SmallStep
   Import CtxNotations.
   Import EnvNotations.
 
-  Inductive Step {Γ : PCtx} {τ : Ty} (γ : RegStore) (μ : Memory) (δ : LocalStore Γ) :
-    forall (γ2 : RegStore) (μ2 : Memory) (δ2 : LocalStore Γ) (s1 s2 : Stm Γ τ), Prop :=
+  Inductive Step {Γ : PCtx} {τ : Ty} (γ : RegStore) (μ : Memory) (δ : CStore Γ) :
+    forall (γ2 : RegStore) (μ2 : Memory) (δ2 : CStore Γ) (s1 s2 : Stm Γ τ), Prop :=
 
   | step_stm_exp
       (e : Exp Γ τ) :
@@ -60,24 +60,24 @@ Module SmallStep
       ⟨ γ , μ , δ, stm_let x σ (stm_fail σ s) k ⟩ ---> ⟨ γ , μ , δ , stm_fail τ s ⟩
   | step_stm_let_step
       (x : 𝑿) (σ : Ty) (s s' : Stm Γ σ) (k : Stm (Γ ▻ (x::σ)) τ)
-      (γ' : RegStore) (μ' : Memory) (δ' : LocalStore Γ) :
+      (γ' : RegStore) (μ' : Memory) (δ' : CStore Γ) :
       ⟨ γ , μ , δ , s ⟩ ---> ⟨ γ' , μ' , δ' , s' ⟩ ->
       ⟨ γ , μ , δ , stm_let x σ s k ⟩ ---> ⟨ γ', μ' , δ' , stm_let x σ s' k ⟩
   | step_stm_block_value
-      (Δ : PCtx) (δΔ : LocalStore Δ) (v : Lit τ) :
+      (Δ : PCtx) (δΔ : CStore Δ) (v : Lit τ) :
       ⟨ γ , μ , δ , stm_block δΔ (stm_lit τ v) ⟩ ---> ⟨ γ , μ , δ , stm_lit τ v ⟩
   | step_stm_block_fail
-      (Δ : PCtx) (δΔ : LocalStore Δ) (s : string) :
+      (Δ : PCtx) (δΔ : CStore Δ) (s : string) :
       ⟨ γ , μ , δ , stm_block δΔ (stm_fail τ s) ⟩ ---> ⟨ γ , μ , δ , stm_fail τ s ⟩
   | step_stm_block_step
-      (Δ : PCtx) (δΔ δΔ' : LocalStore Δ) (k k' : Stm (Γ ▻▻ Δ) τ)
-      (γ' : RegStore) (μ' : Memory) (δ' : LocalStore Γ) :
+      (Δ : PCtx) (δΔ δΔ' : CStore Δ) (k k' : Stm (Γ ▻▻ Δ) τ)
+      (γ' : RegStore) (μ' : Memory) (δ' : CStore Γ) :
       ⟨ γ , μ , δ ►► δΔ , k ⟩ ---> ⟨ γ', μ' , δ' ►► δΔ' , k' ⟩ ->
       ⟨ γ , μ , δ , stm_block δΔ k ⟩ ---> ⟨ γ' , μ' , δ' , stm_block δΔ' k' ⟩
 
   | step_stm_seq_step
       (σ : Ty) (s s' : Stm Γ σ) (k : Stm Γ τ)
-      (γ' : RegStore) (μ' : Memory) (δ' : LocalStore Γ) :
+      (γ' : RegStore) (μ' : Memory) (δ' : CStore Γ) :
       ⟨ γ , μ , δ , s ⟩ ---> ⟨ γ' , μ' , δ' , s' ⟩ ->
       ⟨ γ , μ , δ , stm_seq s k ⟩ ---> ⟨ γ' , μ' , δ' , stm_seq s' k ⟩
   | step_stm_seq_value
@@ -92,21 +92,21 @@ Module SmallStep
       ⟨ γ , μ , δ , stm_call f es ⟩ --->
       ⟨ γ , μ , δ , stm_call_frame (evals es δ) (Pi f) ⟩
   | step_stm_call_frame_step
-      (Δ : PCtx) {δΔ δΔ' : LocalStore Δ} (s s' : Stm Δ τ)
+      (Δ : PCtx) {δΔ δΔ' : CStore Δ} (s s' : Stm Δ τ)
       (γ' : RegStore) (μ' : Memory) :
       ⟨ γ , μ , δΔ , s ⟩ ---> ⟨ γ' , μ' , δΔ' , s' ⟩ ->
       ⟨ γ , μ , δ , stm_call_frame δΔ s ⟩ ---> ⟨ γ' , μ' , δ , stm_call_frame δΔ' s' ⟩
   | step_stm_call_frame_value
-      (Δ : PCtx) {δΔ : LocalStore Δ} (v : Lit τ) :
+      (Δ : PCtx) {δΔ : CStore Δ} (v : Lit τ) :
       ⟨ γ , μ , δ , stm_call_frame δΔ (stm_lit τ v) ⟩ ---> ⟨ γ , μ , δ , stm_lit τ v ⟩
   | step_stm_call_frame_fail
-      (Δ : PCtx) {δΔ : LocalStore Δ} (s : string) :
+      (Δ : PCtx) {δΔ : CStore Δ} (s : string) :
       ⟨ γ , μ , δ , stm_call_frame δΔ (stm_fail τ s) ⟩ ---> ⟨ γ , μ , δ , stm_fail τ s ⟩
-  | step_stm_call_external
+  | step_stm_foreign
       {Δ} {f : 𝑭𝑿 Δ τ} (es : NamedEnv (Exp Γ) Δ) (res : string + Lit τ)
       (γ' : RegStore) (μ' : Memory) :
-      ExternalCall f (evals es δ) res γ γ' μ μ' ->
-      ⟨ γ  , μ  , δ , stm_call_external f es ⟩ --->
+      ForeignCall f (evals es δ) res γ γ' μ μ' ->
+      ⟨ γ  , μ  , δ , stm_foreign f es ⟩ --->
       ⟨ γ' , μ' , δ , match res with
                       | inl msg => stm_fail τ msg
                       | inr v__σ  => stm_lit τ v__σ
@@ -120,7 +120,7 @@ Module SmallStep
       ⟨ γ , μ , δ , stm_assign x (stm_fail τ s) ⟩ ---> ⟨ γ , μ , δ , stm_fail τ s ⟩
   | step_stm_assign_step
       (x : 𝑿) {xInΓ : InCtx (x::τ) Γ} (s s' : Stm Γ τ)
-      (γ' : RegStore) (μ' : Memory) (δ' : LocalStore Γ) :
+      (γ' : RegStore) (μ' : Memory) (δ' : CStore Γ) :
       ⟨ γ , μ , δ , s ⟩ ---> ⟨ γ' , μ' , δ' , s' ⟩ ->
       ⟨ γ , μ , δ , stm_assign x s ⟩ ---> ⟨ γ' , μ' , δ' , stm_assign x s' ⟩
 
@@ -192,7 +192,7 @@ Module SmallStep
 
   | step_stm_bind_step
       (σ : Ty) (s s' : Stm Γ σ) (k : Lit σ -> Stm Γ τ)
-      (γ' : RegStore) (μ' : Memory) (δ' : LocalStore Γ) :
+      (γ' : RegStore) (μ' : Memory) (δ' : CStore Γ) :
       ⟨ γ , μ , δ , s ⟩ ---> ⟨ γ', μ' , δ' , s' ⟩ ->
       ⟨ γ , μ , δ , stm_bind s k ⟩ ---> ⟨ γ', μ' , δ' , stm_bind s' k ⟩
   | step_stm_bind_value
@@ -208,16 +208,16 @@ Module SmallStep
 
   where "⟨ γ1 , μ1 , δ1 , s1 ⟩ ---> ⟨ γ2 , μ2 , δ2 , s2 ⟩" := (@Step _ _ γ1%env μ1%env δ1%env γ2%env μ2%env δ2%env s1%exp s2%exp).
 
-  Inductive Steps {Γ : PCtx} {σ : Ty} (γ1 : RegStore) (μ1 : Memory) (δ1 : LocalStore Γ) (s1 : Stm Γ σ) : RegStore -> Memory -> LocalStore Γ -> Stm Γ σ -> Prop :=
+  Inductive Steps {Γ : PCtx} {σ : Ty} (γ1 : RegStore) (μ1 : Memory) (δ1 : CStore Γ) (s1 : Stm Γ σ) : RegStore -> Memory -> CStore Γ -> Stm Γ σ -> Prop :=
   | step_refl : Steps γ1 μ1 δ1 s1 γ1 μ1 δ1 s1
-  | step_trans {γ2 γ3 : RegStore} {μ2 μ3 : Memory} {δ2 δ3 : LocalStore Γ} {s2 s3 : Stm Γ σ} :
+  | step_trans {γ2 γ3 : RegStore} {μ2 μ3 : Memory} {δ2 δ3 : CStore Γ} {s2 s3 : Stm Γ σ} :
       Step γ1 μ1 δ1 γ2 μ2 δ2 s1 s2 -> Steps γ2 μ2 δ2 s2 γ3 μ3 δ3 s3 -> Steps γ1 μ1 δ1 s1 γ3 μ3 δ3 s3.
 
   Notation "⟨ γ1 , μ1 , δ1 , s1 ⟩ --->* ⟨ γ2 , μ2 , δ2 , s2 ⟩" := (@Steps _ _ γ1 μ1 δ1 s1 γ2 μ2 δ2 s2).
 
-  Inductive StepsN {Γ : PCtx} {σ : Ty} (γ1 : RegStore) (μ1 : Memory) (δ1 : LocalStore Γ) (s1 : Stm Γ σ) : nat -> RegStore -> Memory -> LocalStore Γ -> Stm Γ σ -> Prop :=
+  Inductive StepsN {Γ : PCtx} {σ : Ty} (γ1 : RegStore) (μ1 : Memory) (δ1 : CStore Γ) (s1 : Stm Γ σ) : nat -> RegStore -> Memory -> CStore Γ -> Stm Γ σ -> Prop :=
   | stepsn_refl : StepsN γ1 μ1 δ1 s1 O γ1 μ1 δ1 s1
-  | stepsn_trans {γ2 γ3 : RegStore} {μ2 μ3 : Memory} {δ2 δ3 : LocalStore Γ} {s2 s3 : Stm Γ σ} {n} :
+  | stepsn_trans {γ2 γ3 : RegStore} {μ2 μ3 : Memory} {δ2 δ3 : CStore Γ} {s2 s3 : Stm Γ σ} {n} :
       Step γ1 μ1 δ1 γ2 μ2 δ2 s1 s2 -> StepsN γ2 μ2 δ2 s2 n γ3 μ3 δ3 s3 -> StepsN γ1 μ1 δ1 s1 (S n) γ3 μ3 δ3 s3.
 
   Notation "⟨ γ1 , μ1 , δ1 , s1 ⟩ ---> n ⟨ γ2 , μ2 , δ2 , s2 ⟩" := (@StepsN _ _ γ1 μ1 δ1 s1 n γ2 μ2 δ2 s2).
@@ -251,7 +251,7 @@ Module SmallStep
         end
       | lazymatch head s with
         | @stm_call           => idtac
-        | @stm_call_external  => idtac
+        | @stm_foreign        => idtac
         | @stm_assertk        => idtac
         | @stm_fail           => idtac
         | @stm_exp            => idtac
